cancel_aux proved

cancellation/ElimRel.v
@@ -53,7 +53,12 @@ Section REL.
     arg <- trigger (Choose Any.t);; tau;;
     tid <- trigger (Spawn fn arg);; tau;;
     trigger (Guarantee (ginv' tid -∗ fsp.(precond) tid x varg arg));;; tau;;
-    HoareYieldE ginv' tid;;; tau;;
+    HoareYieldE ginv' tid;;; 
+    Ret tid.
+
+  Definition Spawn_CancelE (fn: gname) (varg: Any.t) : itree hmodE nat :=
+    tid <- trigger (Spawn fn varg);; tau;;
+    trigger (Yield tid);;;
     Ret tid.
 
   Variant elim_rel_def {sk0 A}
@@ -76,27 +81,27 @@ Section REL.
   | elim_rel_core {R} l (e: coreE R) ktrS ktrT
       (KTR: forall (v: R), self l (ktrS v) (ktrT v))
     :
-    elim_rel_def self l (trigger e >>= ktrS) (a <- trigger e;; (tau;; tau;; ktrT a))
+    elim_rel_def self l (trigger e >>= ktrS) (a <- trigger e;; ktrT a)
 
   | elim_rel_pg {R} l (e: pgE R) ktrS ktrT
       (KTR: forall (v: R), self l (ktrS v) (ktrT v))
     :
-    elim_rel_def self l (trigger e >>= ktrS) (a <- trigger e;; (tau;; tau;; ktrT a))
+    elim_rel_def self l (trigger e >>= ktrS) (a <- trigger e;; ktrT a)
 
   | elim_rel_asm P l ktrS ktrT
       (KTR: self l (ktrS tt) (ktrT tt))
     :
-    elim_rel_def self l (trigger (Assume P) >>= ktrS) (a <- trigger (Assume P);; (tau;; tau;; ktrT a))
+    elim_rel_def self l (trigger (Assume P) >>= ktrS) (a <- trigger (Assume P);; ktrT a)
 
   | elim_rel_grt P l ktrS ktrT
       (KTR: self l (ktrS tt) (ktrT tt))
     :
-    elim_rel_def self l (trigger (Guarantee P) >>= ktrS) (a <- trigger (Guarantee P);; (tau;; tau;; ktrT a))
+    elim_rel_def self l (trigger (Guarantee P) >>= ktrS) (a <- trigger (Guarantee P);; ktrT a)
   
   | elim_rel_tid l ktrS ktrT
       (KTR: forall (tid: nat), self l (ktrS tid) (ktrT tid))
     :
-    elim_rel_def self l (trigger Tid >>= ktrS) (a <- trigger Tid;; (tau;; tau;; ktrT a))
+    elim_rel_def self l (trigger Tid >>= ktrS) (a <- trigger Tid;; ktrT a)
 
   | elim_rel_head X P l varg src ktrS ktrT
      (SRC: src = ktrS varg)
@@ -111,7 +116,7 @@ Section REL.
       (KTR: forall vret, self l (ktrS vret) (ktrT vret))
     :
     elim_rel_def self ((tid, tid', existT X (m, m'))::l)
-        (tau;; src) 
+        (tau;; tau;; tau;; src) 
         (x <- @hmod_elim_tail X Q (tid, m, tid', m') vret;; tau;; ktrT x)
         (* (vret' <- (@hmod_elim_tail X Q (tid, m, tid', m') vret);; (tau;; tau;; ktrT vret')) *)
 
@@ -119,14 +124,14 @@ Section REL.
       (STB: stb sk0 fn = Some f)
       (KTR: forall x, self l (ktrS x) (ktrT x))
     :
-    elim_rel_def self l (trigger (Spawn fn args) >>= ktrS)
-                        (x <- HoareSpawnE (ginv sk0) f fn args;; (tau;; ktrT x))
+    elim_rel_def self l (Spawn_CancelE fn args >>= ktrS)
+                        (x <- HoareSpawnE (ginv sk0) f fn args;; ktrT x)
 
   | elim_rel_yield tid l ktrS ktrT
       (KTR: forall x, self l (ktrS x) (ktrT x))
     :
     elim_rel_def self l (trigger (Yield tid) >>= ktrS)
-                        (x <- HoareYieldE (ginv sk0) tid;; (tau;; tau;; ktrT x))
+                        (x <- HoareYieldE (ginv sk0) tid;; ktrT x)
   .
 
   Definition elim_rel {sk0 A} :=
@@ -266,7 +271,7 @@ Section CANCEL.
     :
     inline_hp prog (HoareSpawn ginv' f fn args >>= ktr)
     =
-    x <- HoareSpawnE ginv' f fn args;; inline_hp prog (ktr x).
+    x <- HoareSpawnE ginv' f fn args;; tau;; inline_hp prog (ktr x).
   Proof.
     unfold HoareSpawn, HoareSpawnE. ired.
     rewrite HIRed.bind_core. f_equal. extensionalities. ired. do 2 f_equal.
@@ -274,6 +279,29 @@ Section CANCEL.
     rewrite HIRed.bind_sch. f_equal. extensionalities. ired. do 2 f_equal.
     rewrite HIRed.bind_ag. f_equal. extensionalities. ired. do 2 f_equal.
     rewrite HoareYield_hpI. f_equal. 
+  Qed.
+
+  Lemma Spawn_Cancel_sandbox
+      scopes fn args
+    :
+    HModSem.sandbox scopes (Spawn_Cancel fn args) = Spawn_Cancel fn args.
+  Proof.
+    unfold Spawn_Cancel.
+    rewrite HModSB.transl_bind HModSB.transl_sch. f_equal. extensionalities.
+    rewrite HModSB.transl_bind HModSB.transl_sch. f_equal. extensionalities.
+    rewrite HModSB.transl_ret. ss.
+  Qed. 
+
+  Lemma Spawn_Cancel_hpI
+      prog fn args ktr
+    :
+    inline_hp prog (Spawn_Cancel fn args >>= ktr)
+    =
+    x <- Spawn_CancelE fn args;; tau;; inline_hp prog (ktr x).
+  Proof.
+    unfold Spawn_Cancel, Spawn_CancelE. ired.
+    rewrite HIRed.bind_sch. f_equal. extensionalities. ired. do 2 f_equal.
+    rewrite HIRed.bind_sch. f_equal.
   Qed.
 
   Lemma HoareCall_inline_aux
@@ -405,70 +433,49 @@ Section CANCEL.
     :
     @elim_rel _ ginv stb sk0 _ []
       (inline_hp (prog (SModSemAux.to_hmod (SMod.modsem md sk0))) 
-          (HModSem.sandbox scopes itr))
+          (HModSem.sandbox scopes (interp_smod_aux itr)))
       (inline_hp (prog (SModSem.to_hmod (ginv sk0) (stb sk0) (SMod.modsem md sk0))) 
           (HModSem.sandbox scopes (interp_smod (ginv sk0) (stb sk0) itr))).
   Proof. 
     unfold elim_rel.
     ginit. revert itr scopes. gcofix CIH. i.
     assert (CASE:= case_itrH _ itr). des; subst.
-    - rewrite SModRed.interp_ret HModSB.transl_ret !HIRed.ret.
+    - rewrite SModRed.interp_ret SAuxRed.ret HModSB.transl_ret !HIRed.ret.
       gstep. econs. 
-    - rewrite SModRed.interp_tau !HModSB.transl_tau !HIRed.tau.
+    - rewrite SModRed.interp_tau SAuxRed.tau !HModSB.transl_tau !HIRed.tau.
       gstep; econs. gstep; econs. eauto with paco.
-    - rewrite SModRed.interp_bind SModRed.interp_ag !HModSB.transl_bind HModSB.transl_ag. ired.
-      rewrite !HIRed.bind_ag. 
-      set (fun _ => tau;; _) at 2. eassert (i = _).
-      {
-        unfold i. instantiate (1:= fun _ => tau;; (tau;; tau;; _)).
-        extensionalities. do 2 f_equal.
-        rewrite HModSB.transl_tau HModSB.transl_ret. ired. rewrite HIRed.tau. f_equal.
-      }
-      rewrite H. gstep. econs. gstep. econs. eauto with paco.
-    - rewrite/__ SModRed.interp_bind SModRed.interp_ag !HModSB.transl_bind HModSB.transl_ag. ired.
-      rewrite/__ !HIRed.bind_ag. 
-      set (fun _ => tau;; _) at 2. eassert (i = _).
-      {
-        unfold i. instantiate (1:= fun _ => tau;; (tau;; tau;; _)).
-        extensionalities. do 2 f_equal.
-        rewrite HModSB.transl_tau HModSB.transl_ret. ired. rewrite HIRed.tau. f_equal.
-      }
-      rewrite H. gstep. econs. gstep. econs. eauto with paco.
-    - rewrite/__ SModRed.interp_bind SModRed.interp_sch !HModSB.transl_bind HModSB.transl_sch. ired.
-      unfold handle_schE_hmodE. depdes s.
+    - rewrite SModRed.interp_bind SModRed.interp_ag SAuxRed.bind SAuxRed.ag !HModSB.transl_bind HModSB.transl_ag. ired.
+      rewrite !HIRed.bind_ag. gstep. econs. gstep. econs.
+      rewrite HModSB.transl_tau HModSB.transl_ret. ired. rewrite !HIRed.tau.
+      gstep. econs. gstep. econs. eauto with paco. 
+    - rewrite SModRed.interp_bind SModRed.interp_ag SAuxRed.bind SAuxRed.ag !HModSB.transl_bind HModSB.transl_ag. ired.
+      rewrite !HIRed.bind_ag. gstep. econs. gstep. econs. 
+      rewrite HModSB.transl_tau HModSB.transl_ret. ired. rewrite !HIRed.tau.  
+      gstep. econs. gstep. econs. eauto with paco.
+    - rewrite SModRed.interp_bind SModRed.interp_sch SAuxRed.bind SAuxRed.sch. ired. 
+      unfold handle_schE_hmodE, handle_schE_hmodE_aux. depdes s.
       + destruct (stb sk0 fn) eqn:STB; ired; cycle 1.
         { 
           unfold triggerNB. ired. 
-          rewrite/__ HModSB.transl_bind HModSB.transl_core. ired. 
+          rewrite !HModSB.transl_bind HModSB.transl_core. ired. 
           rewrite HIRed.bind_core. gstep. econs. 
         }
-        rewrite/__ HoareSpawn_sandbox HoareSpawn_hpI HIRed.bind_sch.
-        set (HoareSpawnE _ _ _ _ >>= _). eassert (i = _).
-        {
-          unfold i. instantiate (1:= ITree.bind _ (fun _ => tau;; _)).
-          f_equal. 
-          extensionalities.
-          rewrite HModSB.transl_tau HModSB.transl_ret. ired. 
-          rewrite HIRed.tau. f_equal.
-        }
-        rewrite H. gstep. econs; eauto. i. gstep. econs. eauto with paco.
-      + rewrite/__ HoareYield_sandbox HoareYield_hpI HIRed.bind_sch.
-        set (fun _ => tau;; _) at 2. eassert (i = _).
-        {
-          unfold i. instantiate (1:= fun _ => tau;; (tau;; tau;; _)).
-          extensionalities. do 2 f_equal.
-          rewrite HModSB.transl_tau HModSB.transl_ret. ired. rewrite HIRed.tau. f_equal.
-        }
-        rewrite H. gstep. econs. i. gstep. econs. eauto with paco.
-      + rewrite/__ HModSB.transl_sch !HIRed.bind_sch.
-        set (fun _ => tau;; _) at 2. eassert (i = _).
-        {
-          unfold i. instantiate (1:= fun _ => tau;; (tau;; tau;; _)).
-          extensionalities. do 2 f_equal.
-          rewrite HModSB.transl_tau HModSB.transl_ret. ired. rewrite HIRed.tau. f_equal.
-        }
-        rewrite H. gstep. econs. i. gstep. econs. eauto with paco.
-    - rewrite/__ SModRed.interp_bind SModRed.interp_call.
+        do 2 rewrite HModSB.transl_bind.
+        rewrite HoareSpawn_sandbox HoareSpawn_hpI. 
+        rewrite Spawn_Cancel_sandbox Spawn_Cancel_hpI. ired.
+        gstep. econs; eauto. i. gstep. econs. ired.
+        rewrite !HModSB.transl_tau !HIRed.tau.
+        gstep. econs. gstep. econs. eauto with paco.
+      + do 2 rewrite HModSB.transl_bind. 
+        rewrite HoareYield_sandbox HoareYield_hpI HModSB.transl_sch HIRed.bind_sch.
+        gstep. econs. i. gstep. econs. ired.
+        rewrite !HModSB.transl_tau !HIRed.tau.
+        gstep. econs. gstep. econs. eauto with paco.
+      + rewrite !HModSB.transl_bind HModSB.transl_sch !HIRed.bind_sch.
+        gstep. econs. gstep. econs. ired.
+        rewrite !HModSB.transl_tau !HIRed.tau.
+        gstep. econs. gstep. econs. eauto with paco.
+    - rewrite SModRed.interp_bind SModRed.interp_call SAuxRed.bind SAuxRed.call.
       unfold handle_callE_hmodE. depdes c. 
       destruct (stb sk0 fn) eqn: STB; ired; cycle 1.
       { 
@@ -477,22 +484,24 @@ Section CANCEL.
         rewrite HIRed.bind_core. gstep. econs.
       }
       do 2 rewrite HModSB.transl_bind. 
-      rewrite/__ HModSB.transl_call HIRed.call HIRed.bind.
+      rewrite HModSB.transl_call HIRed.call HIRed.bind.
       
       assert (FIND := stb_in_alist_find).
       specialize (FIND sk0 fn f SKINCL SKWF STB). des.
-      destruct (alist_find fn (List.map (map_snd (λ ksb : list string * fspecbody, (ksb.1, fsb_body ksb.2))) (SModSem.fnsems (SMod.modsem md sk0)))) eqn: FINDS; cycle 1.
+      destruct (alist_find fn (List.map (map_snd (λ ksb : list string * fspecbody, (ksb.1, interp_sb_hp_aux ksb.2))) (SModSem.fnsems (SMod.modsem md sk0)))) eqn: FINDS; cycle 1.
       { exfalso. rewrite/__ alist_find_map_snd FIND in FINDS. clarify.  }
-      ired. rewrite FINDS. destruct p. rewrite/__ alist_find_map_snd FIND in FINDS. s in FINDS. inv FINDS. 
+      ired. rewrite FINDS. destruct p. rewrite alist_find_map_snd FIND in FINDS. s in FINDS. inv FINDS. 
       ired. unfold HModSem.sandbox_body. s. 
       set_l. 
-      eassert (ITREE = tau;; x <- (a <- inline_hp _ (HModSem.sandbox l0 (i args));; tau;; Ret a);; tau;; _).
+      eassert (ITREE = tau;; x <- (a <- inline_hp _ (HModSem.sandbox l0 (x <- _ args;; tau;; Ret x));; tau;; Ret a);; tau;; _).
       {
         unfold ITREE. do 2 f_equal. 
-        instantiate (2:= prog (SModSemAux.to_hmod (SMod.modsem md sk0))).
-        ired. f_equal.  
-        extensionalities. rewrite HIRed.tau. ired.
+        instantiate (3:= prog (SModSemAux.to_hmod (SMod.modsem md sk0))).
+        ired. rewrite HModSB.transl_bind HIRed.bind. ired. f_equal.  
+        extensionalities. rewrite HModSB.transl_tau !HIRed.tau. ired.
         do 4 f_equal.
+        rewrite HModSB.transl_ret HIRed.ret. ired.
+        rewrite HModSB.transl_tau HIRed.tau. do 4 f_equal.
       }
       set_r.
       eassert (ITREE0 = x <- (a <- inline_hp _ _;; tau;; Ret a);; tau;; _ x).
@@ -511,19 +520,22 @@ Section CANCEL.
       rewrite -bind_tau. guclo elim_rel_bindC_spec. econs.
       {
         erewrite HoareCall_inline; eauto.
-        set (inline_hp _ _ ). eassert (i0 = _ args).
-        {
-          unfold i0. instantiate (1:= fun x => inline_hp _ (_ ( i x))).
-          refl.
-        }
-        remember (λ x : Any.t, inline_hp (prog (SModSemAux.to_hmod (SMod.modsem md sk0))) (HModSem.sandbox l0 (i x))).
-        rewrite H. clear i0 H.
+        rewrite HModSB.transl_bind HIRed.bind.
+        set (inline_hp _ _ ). eassert (i = _ args).
+        { unfold i. instantiate (1:= fun x => inline_hp _ (_ (_ x))). refl. }
+        remember (λ x : Any.t, inline_hp (prog (SModSemAux.to_hmod (SMod.modsem md sk0))) (HModSem.sandbox l0 (_ x))).
+        rewrite H. clear i H.
         ired. gstep. econs. 
-        { instantiate (1:= fun args => a <- i1 args;; tau;; Ret a). s. refl. }
+        { 
+          instantiate (1:= fun args => a <- i0 args;; tau;; tau;; tau;; Ret a). s. 
+          f_equal. extensionalities.
+          rewrite HModSB.transl_tau HModSB.transl_ret HIRed.tau HIRed.ret.
+          ired. refl. 
+        }
         i. ired. 
         (* rewrite [i1 varg]add_dummy_ret. *)
         guclo elim_rel_bindC_spec. econs.
-        { rewrite Heqi1. eauto with paco. }
+        { rewrite Heqi0. unfold interp_sb_hp_aux. s. eauto with paco. }
         i.
         set_r. eassert (ITREE = a <- hmod_elim_tail (meta f) (postcond f) (tid, m, tid', m') v;; (tau;; Ret a)).
         { unfold ITREE, hmod_elim_tail. refl. }
@@ -535,51 +547,37 @@ Section CANCEL.
       i. gstep. econs. eauto with paco.
 
     - depdes s.
-      + rewrite/__ SModRed.interp_bind SModRed.interp_pg !HModSB.transl_bind HModSB.transl_put. ired.
+      + rewrite SModRed.interp_bind SModRed.interp_pg SAuxRed.bind SAuxRed.pg. 
+        rewrite !HModSB.transl_bind HModSB.transl_put. ired.
         des_ifs.
-        * rewrite/__ !HIRed.bind_pg.
-          set (fun _ => tau;; _) at 2. eassert (i = _).
-          {
-            unfold i. instantiate (1:= fun _ => tau;; (tau;; tau;; _)).
-            extensionalities. do 2 f_equal.
-            rewrite HModSB.transl_tau HModSB.transl_ret. ired. rewrite HIRed.tau. f_equal.
-          }
-          rewrite H. gstep. econs. i. gstep. econs. eauto with paco. 
-        * rewrite/__ !HIRed.bind_core.
-          set (fun _ => tau;; _) at 2. eassert (i = _).
-          {
-            unfold i. instantiate (1:= fun _ => tau;; (tau;; tau;; _)).
-            extensionalities. do 2 f_equal.
-            rewrite HModSB.transl_tau HModSB.transl_ret. ired. rewrite HIRed.tau. f_equal.
-          } 
-          rewrite H. gstep. econs. i. gstep. econs. eauto with paco. 
-      + rewrite/__ SModRed.interp_bind SModRed.interp_pg !HModSB.transl_bind HModSB.transl_get. ired.
+        * rewrite !HIRed.bind_pg.
+          gstep. econs. i. gstep. econs.
+          rewrite HModSB.transl_tau HModSB.transl_ret. ired.
+          rewrite !HIRed.tau.
+          gstep. econs. i. gstep. econs. eauto with paco. 
+        * rewrite !HIRed.bind_core.
+          gstep. econs. i. gstep. econs.
+          rewrite HModSB.transl_tau HModSB.transl_ret. ired.
+          rewrite !HIRed.tau.
+          gstep. econs. i. gstep. econs. eauto with paco.  
+      + rewrite SModRed.interp_bind SModRed.interp_pg SAuxRed.bind SAuxRed.pg. 
+        rewrite !HModSB.transl_bind HModSB.transl_get. ired.
         des_ifs.
-        * rewrite/__ !HIRed.bind_pg. 
-          set (fun _ => tau;; _) at 2. eassert (i = _).
-          {
-            unfold i. instantiate (1:= fun _ => tau;; (tau;; tau;; _)).
-            extensionalities. do 2 f_equal.
-            rewrite HModSB.transl_tau HModSB.transl_ret. ired. rewrite HIRed.tau. f_equal.
-          } 
-          rewrite H. gstep. econs. i. gstep. econs. eauto with paco.
-        * rewrite/__ !HIRed.bind_core. 
-          set (fun _ => tau;; _) at 2. eassert (i = _).
-          {
-            unfold i. instantiate (1:= fun _ => tau;; (tau;; tau;; _)).
-            extensionalities. do 2 f_equal.
-            rewrite HModSB.transl_tau HModSB.transl_ret. ired. rewrite HIRed.tau. f_equal.
-          } 
-          rewrite H. gstep. econs. i. gstep. econs. eauto with paco. 
-    - rewrite/__ SModRed.interp_bind SModRed.interp_core !HModSB.transl_bind HModSB.transl_core. ired.
-      rewrite/__ !HIRed.bind_core. 
-      set (fun _ => tau;; _) at 2. eassert (i = _).
-      {
-        unfold i. instantiate (1:= fun _ => tau;; (tau;; tau;; _)).
-        extensionalities. do 2 f_equal.
-        rewrite HModSB.transl_tau HModSB.transl_ret. ired. rewrite HIRed.tau. f_equal.
-      }   
-      rewrite H. gstep. econs. i. gstep. econs. eauto with paco. 
+        * rewrite !HIRed.bind_pg.
+          gstep. econs. i. gstep. econs.
+          rewrite HModSB.transl_tau HModSB.transl_ret. ired.
+          rewrite !HIRed.tau.
+          gstep. econs. i. gstep. econs. eauto with paco. 
+        * rewrite !HIRed.bind_core.
+          gstep. econs. i. gstep. econs.
+          rewrite HModSB.transl_tau HModSB.transl_ret. ired.
+          rewrite !HIRed.tau.
+          gstep. econs. i. gstep. econs. eauto with paco.  
+    - rewrite SModRed.interp_bind SModRed.interp_core SAuxRed.bind SAuxRed.core. ired. 
+      rewrite !HModSB.transl_bind HModSB.transl_core !HIRed.bind_core. 
+      gstep. econs. i. gstep. econs. ired. 
+      rewrite !HModSB.transl_tau !HIRed.tau.
+      gstep. econs. i. gstep. econs. eauto with paco.
   Qed.
 
 End CANCEL.
